LinearSTLC bugs

src/Pyrosome/Lang/LinearSTLC.v
@@ -6,7 +6,7 @@ Import ListNotations.
 Open Scope string.
 Open Scope list.
 From Utils Require Import Utils.
-From Pyrosome Require Import Theory.Core Elab.Elab Tools.Matches Lang.SimpleVSubst.
+From Pyrosome Require Import Theory.Core Elab.Elab Tools.Matches Lang.LinearSubst.
 Import Core.Notations.
 
 Require Coq.derive.Derive.
@@ -80,17 +80,18 @@ Definition linear_stlc_def : lang :=
       : #"exp" (#"conc" "G" "H") "B"
   ];
 
-  [:= "G" : #"env",
+  [:= "G" : #"env", "H" : #"env",
       "A" : #"ty",
       "B" : #"ty",
       "e" : #"exp" "G" (#"lolli" "A" "B"),
-      "e'" : #"exp" "G" "A",
-      "G'" : #"env",
-      "g" : #"sub" "G'" "G"
+      "e'" : #"exp" "H" "A",
+      "G'" : #"env", "H'" : #"env",
+      "g" : #"sub" "G'" "G",
+      "h" : #"sub" "H'" "H"
       ----------------------------------------------- ("linear_app-subst")
-      #"exp_subst" "g" (#"linear_app" "e" "e'")
-       = #"linear_app" (#"exp_subst" "g" "e") (#"exp_subst" "g" "e'")
-       : #"exp" "G'" "B"
+      #"exp_subst" (#"csub" "g" "h") (#"linear_app" "e" "e'")
+       = #"linear_app" (#"exp_subst" "g" "e") (#"exp_subst" "h" "e'")
+       : #"exp" (#"conc" "G'" "H'") "B"
   ];
   [:= "G" : #"env",
       "A" : #"ty",
@@ -100,15 +101,52 @@ Definition linear_stlc_def : lang :=
       "g" : #"sub" "G'" "G"
       ----------------------------------------------- ("linear_lambda-subst")
       #"val_subst" "g" (#"linear_lambda" "A" "e")
-      = #"linear_lambda" "A" (#"exp_subst" (#"csub" "g" #"id") "e")
+      = #"linear_lambda" "A" (#"exp_subst" (#"snoc" "g" #"hd") "e")
       : #"val" "G'" (#"lolli" "A" "B")
   ]
   ]}.
 
-Derive stlc
-       SuchThat (elab_lang_ext (exp_subst++value_subst) [] (* stlc_def *) stlc)
-       As stlc_wf.
-Proof. auto_elab. Qed.
-#[export] Hint Resolve stlc_wf : elab_pfs.
+Derive linear_stlc
+       SuchThat (elab_lang_ext (linear_exp_subst++linear_value_subst) linear_stlc_def linear_stlc)
+       As linear_stlc_wf.
+Proof. setup_elab_lang.
+- break_elab_rule.
+- break_elab_rule.
+- break_elab_rule.
+- break_elab_rule.
+- eapply eq_term_rule.
+  + break_down_elab_ctx.
+  + break_elab_sort.
+  + eapply elab_term_conv.
+      -- eapply elab_term_by.
+        ++ solve_in.
+        ++ eapply elab_args_cons_ex'.
+           { solve_len_eq. }
+           { cbn_elab_goal.
+              eapply elab_term_conv.
+              { eapply elab_term_by.
+                { solve_in. }
+                eapply elab_args_cons_ex'.
+                { solve_len_eq. }
+                { cbn_elab_goal.
+                  try_break_elab_term. }
+                eapply elab_args_cons_ex'.
+                { solve_len_eq. }
+                { (* try_break_elab_term (* this should work *) *)
+                  cbn_elab_goal.
+                  eapply elab_term_var.
+                  solve_in. }
+                 break_down_elab_args. }
+            compute_eq_compilation.
+            sort_cong.
+            { (* process_eq_term. *) (* fails *)
+              term_refl. }
+            process_eq_term. }
+            eapp
+      -- solve_in.
+      -- eapply elab_args_cons_ex'.
+         2: try_break_elab_term.
+     Qed.
+#[export] Hint Resolve linear_stlc_wf : elab_pfs.
 
 
